rocq_proofs/memory_model.v
@@ -7,240 +7,239 @@ Set Implicit Arguments.
 
 Module ConcreteValue <: ValueSig.
 
-Definition t := value.
-Definition eq_dec := value_eq_dec.
+  Definition t := value.
+  Definition eq_dec := value_eq_dec.
 
-(* IMM gives every location an initial write.  We interpret that write as
-   saying that the location has not yet been allocated. *)
-Definition init : t := VUnalloc.
+  (* IMM gives every location an initial write.  We interpret that write as
+    saying that the location has not yet been allocated. *)
+  Definition init : t := VUnalloc.
 
 End ConcreteValue.
 
 Module MemoryModel
     (Ev : Events ConcreteValue).
 
-Module Import Ex := Execution ConcreteValue Ev.
+  Module Import Ex := Execution ConcreteValue Ev.
 
-Definition read_label
-    (x : Ev.location) (ord : Ev.mode) (v : ConcreteValue.t) : Ev.label :=
-  Ev.Aload false ord x v.
+  Definition read_label
+      (x : Ev.location) (ord : Ev.mode) (v : ConcreteValue.t) : Ev.label :=
+    Ev.Aload false ord x v.
 
-Definition write_label
-    (x : Ev.location) (ord : Ev.mode) (v : ConcreteValue.t) : Ev.label :=
-  Ev.Astore Ev.Xpln ord x v.
+  Definition write_label
+      (x : Ev.location) (ord : Ev.mode) (v : ConcreteValue.t) : Ev.label :=
+    Ev.Astore Ev.Xpln ord x v.
 
 Inductive memory_action : Type :=
-| MRead      : Ev.location -> Ev.mode -> ConcreteValue.t -> memory_action
-| MWrite     : Ev.location -> Ev.mode -> ConcreteValue.t -> memory_action
-| MReadFail  : Ev.location -> memory_action
-| MWriteFail : Ev.location -> memory_action
-| MMalloc    : Ev.location -> memory_action
-| MFree      : Ev.location -> memory_action.
+| MRead      : Ev.thread_id -> Ev.location -> Ev.mode -> ConcreteValue.t -> memory_action
+| MWrite     : Ev.thread_id -> Ev.location -> Ev.mode -> ConcreteValue.t -> memory_action
+| MReadFail  : Ev.thread_id -> Ev.location -> memory_action
+| MWriteFail : Ev.thread_id -> Ev.location -> memory_action
+| MMalloc    : Ev.thread_id -> Ev.location -> memory_action
+| MFree      : Ev.thread_id -> Ev.location -> memory_action.
 
-Record extends_execution
-    (G G' : execution) (e : Ev.actid) : Prop := {
-  extends_G': acts_set G' e; 
-  extends_fresh :
-    ~ acts_set G e;
-  extends_acts :
-    forall a, acts_set G' a <-> acts_set G a \/ a = e;
-  extends_lab :
-    forall a, acts_set G a -> lab G' a = lab G a;
-  extends_sb :
-    forall a,
-      acts_set G a ->
-      Ev.tid a = Ev.tid e ->
-      Ev.ext_sb a e
-}.
-    
-Definition coherence_maximal_write (G: execution) (x: Ev.location) := fun w =>
-  acts_set G w /\
-  Ev.is_w (lab G) w = true /\
-  Ev.loc (lab G) w = Some x /\
-  ~ exists w',
-      acts_set G w' /\
-      Ev.is_w (lab G) w' = true /\
-      co G w w'
-.
+  Record extends_execution
+      (G G' : execution) (e : Ev.actid) : Prop := {
+    extends_G': acts_set G' e; 
+    extends_fresh :
+      ~ acts_set G e;
+    extends_acts :
+      forall a, acts_set G' a <-> acts_set G a \/ a = e;
+    extends_lab :
+      forall a, acts_set G a -> lab G' a = lab G a;
+    extends_sb :
+      forall a,
+        acts_set G a ->
+        Ev.tid a = Ev.tid e ->
+        Ev.ext_sb a e
+  }.
+      
+  Definition coherence_maximal_write (G: execution) (x: Ev.location) := fun w =>
+    acts_set G w /\
+    Ev.is_w (lab G) w = true /\
+    Ev.loc (lab G) w = Some x /\
+    ~ exists w',
+        acts_set G w' /\
+        Ev.is_w (lab G) w' = true /\
+        co G w w'
+  .
 
-Definition isAllocated (G : execution) (x : Ev.location) : Prop :=
-  exists w v,
-    coherence_maximal_write G x w /\
-    Ev.val (lab G) w = Some v /\
-    v <> VUnalloc.
+  Definition isAllocated (G : execution) (x : Ev.location) : Prop :=
+    exists w v,
+      coherence_maximal_write G x w /\
+      Ev.val (lab G) w = Some v /\
+      v <> VUnalloc.
 
-Definition neverAllocated (G : execution) (x : Ev.location): Prop :=   ~ (isAllocated G x). 
+  Definition neverAllocated (G : execution) (x : Ev.location): Prop :=   ~ (isAllocated G x). 
 
-(* A memory model is the model-specific consistency predicate over the
-   execution graphs shared by IMM, RC11, Arm, etc. *)
-Record t := {
-  consistent : execution -> Prop;
-  consistent_complete :
-    forall G, consistent G -> complete G
-}.
+  (* A memory model is the model-specific consistency predicate over the
+    execution graphs shared by IMM, RC11, Arm, etc. *)
+  Record t := {
+    consistent : execution -> Prop;
+    consistent_complete :
+      forall G, consistent G -> complete G
+  }.
 
-(* Model consistency and structural well-formedness are deliberately kept
-   separate in the adapters.  In the imported development, for example,
-   [imm_consistent] and [rc11_consistent] do not contain [Wf], whereas
-   [ArmConsistent] does.  Generic transitions use the normalized judgment
-   below. *)
-Definition valid_execution (M : t) (G : execution) : Prop :=
-  Wf G  /\ consistent M G.
+  Section WithModel.
 
+  Context (M : t).
 
-Inductive memory_step (M : t) : execution -> memory_action -> execution -> Prop :=
-| Step_MRead :
-    forall G G' e x ty v,
-      valid_execution M G ->
-      extends_execution G G' e ->
-      lab G' e = read_label x ty v ->
-      v <> VUnalloc ->
-      valid_execution M G' ->
-
-      memory_step M G (MRead x ty v) G'
-
-| Step_MWrite :
-    forall G G' e x ty v,
-      valid_execution M G ->
-      isAllocated G x ->
-      extends_execution G G' e ->
-      lab G' e = write_label x ty v ->
-      valid_execution M G' ->
-
-      memory_step M G (MWrite x ty v) G'
-
-| Step_MReadFail :
-    forall G G' e x ty,
-      valid_execution M G ->
-      ~ isAllocated G x ->
-      extends_execution G G' e ->
-      lab G' e = read_label x ty VUnalloc ->
-      valid_execution M G' ->
-
-      memory_step M G (MReadFail x) G'
-
-| Step_MWriteFail :
-    forall G G' e x ty v,
-      valid_execution M G ->
-      ~ isAllocated G x ->
-      extends_execution G G' e ->
-      lab G' e = write_label x ty v ->
-      valid_execution M G' ->
-
-      memory_step M G (MWriteFail x) G'
-
-| Step_MMalloc :
-    forall G G' e x ty,
-      valid_execution M G ->
-      neverAllocated G x ->
-      extends_execution G G' e ->
-      lab G' e = write_label x ty VUndef ->
-      valid_execution M G' ->
-
-      memory_step M G (MMalloc x) G'
-
-| Step_MFree :
-    forall G G' e x ty,
-      valid_execution M G ->
-      isAllocated G x ->
-      extends_execution G G' e ->
-      lab G' e = write_label x ty VUnalloc ->
-      valid_execution M G' ->
-
-      memory_step M G (MFree x) G'.
+  (* Model consistency and structural well-formedness are deliberately kept
+    separate in the adapters.  In the imported development, for example,
+    [imm_consistent] and [rc11_consistent] do not contain [Wf], whereas
+    [ArmConsistent] does.  Generic transitions use the normalized judgment
+    below. *)
+  Definition valid_execution (G : execution) : Prop :=
+    Wf G  /\ consistent M G.
 
 
+  Inductive memory_step : execution -> memory_action -> execution -> Prop :=
+  | Step_MRead :
+      forall G G' e thread x ty v,
+        valid_execution G ->
+        extends_execution G G' e ->
+        Ev.tid e = thread ->
+        lab G' e = read_label x ty v ->
+        v <> VUnalloc ->
+        valid_execution G' ->
 
-Lemma extends_is_w
-    G G' e x
-    (EXT : extends_execution G G' e)
-    (IN : acts_set G x) :
-  Ev.is_w (lab G') x = true ->
-  Ev.is_w (lab G) x = true.
-Proof.
-  intro W.
-  unfold Ev.is_w in W.
-  rewrite (extends_lab EXT x IN) in W.
-  exact W.
-Qed.
+        memory_step G (MRead thread x ty v) G'
 
-Lemma extends_execution_R: 
-  forall M G G' e x ty v, 
-    memory_step M G (MRead x ty v) G' -> 
-      extends_execution G G' e -> 
-      exists e0, 
-        acts_set G e0 /\ 
-        Ev.is_w (lab G) e0 = true /\ 
-        rf G' e0 e.  
-Proof with eauto. 
-intros. 
-inversion H. subst.  
-assert (E_EQ : e = e0). {
-  pose proof (extends_G' H5) as E0_IN_G'.
-  apply (extends_acts H0 e0) in E0_IN_G'.
-  destruct E0_IN_G' as [E0_IN_G | E0_EQ].
-  - exfalso.
-    exact (extends_fresh H5 E0_IN_G).
-  - symmetry.
-    exact E0_EQ.
-}
-subst e.
-unfold valid_execution in H10. 
-destruct H10 as [WF CONS].  
-pose proof
-  (consistent_complete M G' CONS)
-  as COMPLETE_G'. 
-unfold complete in COMPLETE_G'.  
-unfold set_inter in COMPLETE_G'. 
-unfold set_subset in COMPLETE_G'. 
-specialize COMPLETE_G' with e0.    
-pose proof (extends_fresh H5) as FRESH. 
-pose proof (extends_acts H5 e0) as ACTS. 
-assert (acts_set G' e0 /\ Ev.is_r (lab G') e0). {
-  split.  
-  assert (e0 = e0) by reflexivity. 
-  assert (acts_set G e0 \/ e0 = e0). {right...  }
-  rewrite <- ACTS in H2... 
-  unfold read_label in H7. 
-  unfold Ev.is_r. rewrite H7...        
-} 
-apply COMPLETE_G' in H1.  
-unfold codom_rel in H1. destruct H1 as [x0 RF].      
-pose proof RF as RF_TYPED. 
-apply (wf_rfD WF) in RF_TYPED. 
-unfolder in RF_TYPED. 
-destruct RF_TYPED as [W _].
-pose proof (extends_acts H5 x0) as ACTS_X0. 
-assert (X0_IN_G' : acts_set G' x0). {
-  pose proof RF as RF_IN_G'.
-  apply (wf_rfE WF) in RF_IN_G'.
-  unfolder in RF_IN_G'.
-  desf.
-}
-assert (X0_NE : x0 <> e0). {
-  intro EQ.
-  subst x0.
-  unfold Ev.is_w in W.
-  rewrite H7 in W.
-  unfold read_label in W.
-  discriminate.
-}
-assert (X0_IN_G : acts_set G x0). {
-  apply ACTS_X0 in X0_IN_G'.
-  destruct X0_IN_G' as [OLD | NEW].
-  - exact OLD.
-  - exfalso.
-    apply X0_NE.
-    exact NEW.
-}
-pose proof
-  (@extends_is_w G G' e0 x0 H5 X0_IN_G W)
-  as W_OLD.
-exists x0.
-repeat split.
-- exact X0_IN_G.
-- exact W_OLD.
-- exact RF.
-Qed.
+  | Step_MWrite :
+      forall G G' e thread x ty v,
+        valid_execution G ->
+        isAllocated G x ->
+        extends_execution G G' e ->
+        Ev.tid e = thread ->
+        lab G' e = write_label x ty v ->
+        valid_execution G' ->
+
+        memory_step G (MWrite thread x ty v) G'
+
+  | Step_MReadFail :
+      forall G G' e thread x ty,
+        valid_execution G ->
+        ~ isAllocated G x ->
+        extends_execution G G' e ->
+        Ev.tid e = thread ->
+        lab G' e = read_label x ty VUnalloc ->
+        valid_execution G' ->
+
+        memory_step G (MReadFail thread x) G'
+
+  | Step_MWriteFail :
+      forall G G' e thread x ty v,
+        valid_execution G ->
+        ~ isAllocated G x ->
+        extends_execution G G' e ->
+        Ev.tid e = thread ->
+        lab G' e = write_label x ty v ->
+        valid_execution G' ->
+
+        memory_step G (MWriteFail thread x) G'
+
+  | Step_MMalloc :
+      forall G G' e thread x ty,
+        valid_execution G ->
+        neverAllocated G x ->
+        extends_execution G G' e ->
+        Ev.tid e = thread ->
+        lab G' e = write_label x ty VUndef ->
+        valid_execution G' ->
+
+        memory_step G (MMalloc thread x) G'
+
+  | Step_MFree :
+      forall G G' e thread x ty,
+        valid_execution G ->
+        isAllocated G x ->
+        extends_execution G G' e ->
+        Ev.tid e = thread ->
+        lab G' e = write_label x ty VUnalloc ->
+        valid_execution G' ->
+
+        memory_step G (MFree thread x) G'.
+
+
+
+  Lemma extends_is_w
+      G G' e x
+      (EXT : extends_execution G G' e)
+      (IN : acts_set G x) :
+    Ev.is_w (lab G') x = true ->
+    Ev.is_w (lab G) x = true.
+  Proof.
+    intro W.
+    unfold Ev.is_w in W.
+    rewrite (extends_lab EXT x IN) in W.
+    exact W.
+  Qed.
+
+  Lemma extends_execution_R: 
+    forall G G' e thread x ty v,
+      memory_step G (MRead thread x ty v) G' ->
+        extends_execution G G' e -> 
+        exists e0, 
+          acts_set G e0 /\ 
+          Ev.is_w (lab G) e0 = true /\ 
+          rf G' e0 e.  
+  Proof with eauto. 
+    intros. 
+    inversion H. subst.  
+    assert (E_EQ : e = e0). {
+      pose proof (extends_G' H6) as E0_IN_G'.
+      apply (extends_acts H0 e0) in E0_IN_G'.
+      destruct E0_IN_G' as [E0_IN_G | E0_EQ]...  
+      exfalso. exact (extends_fresh H6 E0_IN_G).
+    } 
+    subst e.
+    unfold valid_execution in H12.
+    destruct H12 as [WF CONS].
+    pose proof (consistent_complete M G' CONS) as COMPLETE_G'. 
+    unfold complete in COMPLETE_G'.  
+    unfold set_inter in COMPLETE_G'. 
+    unfold set_subset in COMPLETE_G'. 
+    specialize COMPLETE_G' with e0.    
+    pose proof (extends_fresh H6) as FRESH.
+    pose proof (extends_acts H6 e0) as ACTS.
+    assert (acts_set G' e0 /\ Ev.is_r (lab G') e0). {
+      split.  
+      assert (e0 = e0) by reflexivity. 
+      assert (acts_set G e0 \/ e0 = e0). {right...  }
+      rewrite <- ACTS in H2... 
+      unfold read_label in H10.
+      unfold Ev.is_r. rewrite H10...
+    } 
+    apply COMPLETE_G' in H1.  
+    unfold codom_rel in H1. destruct H1 as [x0 RF].      
+    pose proof RF as RF_TYPED. 
+    apply (wf_rfD WF) in RF_TYPED. 
+    unfolder in RF_TYPED. 
+    destruct RF_TYPED as [W _].
+    pose proof (extends_acts H6 x0) as ACTS_X0.
+    assert (X0_IN_G' : acts_set G' x0). {
+      pose proof RF as RF_IN_G'.
+      apply (wf_rfE WF) in RF_IN_G'.
+      unfolder in RF_IN_G'.
+      desf.
+    }
+    assert (X0_NE : x0 <> e0). {
+      intro EQ.
+      subst x0.
+      unfold Ev.is_w in W.
+      rewrite H10 in W.
+      unfold read_label in W.
+      discriminate.
+    }
+    assert (X0_IN_G : acts_set G x0). {
+      apply ACTS_X0 in X0_IN_G'.
+      destruct X0_IN_G' as [OLD | NEW]... 
+      exfalso. apply X0_NE. exact NEW.
+    } 
+    pose proof (@extends_is_w G G' e0 x0 H6 X0_IN_G W) as W_OLD.
+    exists x0. 
+    repeat split...  
+  Qed.
+
+  End WithModel.
 
 End MemoryModel.
