rocq_proofs/mem_comp.v
@@ -1,0 +1,227 @@
+From hahn Require Import Hahn.
+
+Require Import Events.
+Require Import Execution.
+Require Import value.
+
+Require Import memory_model.
+Require Import thread_semantics.
+
+Set Implicit Arguments.
+
+
+Module Composition (Ev : Events ConcreteValue).
+
+  Module Import MM := MemoryModel Ev.
+  Module Import Ex := MM.Ex.
+
+  Module WholeSystem (S : ThreadSemantics Ev).
+
+    Definition thread_pool : Type := Ev.thread_id -> option S.state.
+
+    Parameter thread_id_eq_dec :  forall x y : Ev.thread_id, {x = y} + {x <> y}.
+
+    Definition update_thread (thread : Ev.thread_id) (state : option S.state) (threads : thread_pool) : thread_pool :=
+      fun thread' => if thread_id_eq_dec thread' thread then state else threads thread'. 
+
+    Definition add_thread (thread : Ev.thread_id) (state : S.state) (threads : thread_pool) : thread_pool :=
+      update_thread thread (Some state) threads.
+
+    Definition remove_thread (thread : Ev.thread_id) (threads : thread_pool) : thread_pool :=
+      update_thread thread None threads.
+
+
+    Record system_state : Type := {
+      sys_graph : execution;
+      sys_threads : thread_pool
+    }.
+
+
+    Inductive system_event : Type :=
+    | WSTau :
+        system_event
+
+    | WSExternal :
+        S.external_event ->
+        system_event
+
+    | WSFail :
+        system_event.
+
+    Section WithMemoryModel.
+
+    Context (M : MM.t).
+
+
+    Inductive system_step : system_state -> system_event -> system_state -> Prop :=
+    | Step_Tau : forall G threads thread state state',
+          threads thread = Some state -> S.step S.globalenv state S.TETau state' ->
+          system_step
+            {|
+              sys_graph := G;
+              sys_threads := threads
+            |}
+            WSTau
+            {|
+              sys_graph := G;
+              sys_threads := update_thread thread (Some state') threads
+            |}
+    | Step_External : forall G threads thread state state' event,
+          threads thread = Some state -> S.step S.globalenv state (S.TEExternal event) state' ->
+              system_step
+                {|
+                  sys_graph := G;
+                  sys_threads := threads
+                |}
+                (WSExternal event)
+                {|
+                  sys_graph := G;
+                  sys_threads :=
+                    update_thread
+                      thread
+                      (Some state')
+                      threads
+                |}
+    | Step_Read :
+        forall G G' threads thread state state' x ord v,
+          threads thread = Some state ->
+          S.step S.globalenv state (S.TEMemory (S.MemoryEvents.TERead x ord v)) state' ->
+          MM.memory_step M G (MM.MRead thread x ord v) G' ->
+          system_step
+            {| sys_graph := G; sys_threads := threads |}
+            WSTau
+            {| sys_graph := G';
+               sys_threads := update_thread thread (Some state') threads |}
+
+    | Step_ReadFail :
+        forall G G' threads thread state state' x ord v,
+          threads thread = Some state ->
+          S.step S.globalenv state (S.TEMemory (S.MemoryEvents.TERead x ord v)) state' ->
+          MM.memory_step M G (MM.MReadFail thread x) G' ->
+          system_step
+            {| sys_graph := G; sys_threads := threads |}
+            WSFail
+            {| sys_graph := G';
+               sys_threads := update_thread thread (Some state') threads |}
+
+    | Step_Write :
+        forall G G' threads thread state state' x ord v,
+          threads thread = Some state ->
+          S.step S.globalenv state (S.TEMemory (S.MemoryEvents.TEWrite x ord v)) state' ->
+          MM.memory_step M G (MM.MWrite thread x ord v) G' ->
+          system_step
+            {| sys_graph := G; sys_threads := threads |}
+            WSTau
+            {| sys_graph := G';
+               sys_threads := update_thread thread (Some state') threads |}
+
+    | Step_WriteFail :
+        forall G G' threads thread state state' x ord v,
+          threads thread = Some state ->
+          S.step S.globalenv state (S.TEMemory (S.MemoryEvents.TEWrite x ord v)) state' ->
+          MM.memory_step M G (MM.MWriteFail thread x) G' ->
+          system_step
+            {| sys_graph := G; sys_threads := threads |}
+            WSFail
+            {| sys_graph := G';
+               sys_threads := update_thread thread (Some state') threads |}
+
+    | Step_Malloc :
+        forall G G' threads thread state state' x,
+          threads thread = Some state ->
+          S.step S.globalenv state (S.TEMemory (S.MemoryEvents.TEMalloc x)) state' ->
+          MM.memory_step M G (MM.MMalloc thread x) G' ->
+          system_step
+            {| sys_graph := G; sys_threads := threads |}
+            WSTau
+            {| sys_graph := G';
+               sys_threads := update_thread thread (Some state') threads |}
+
+    | Step_Free :
+        forall G G' threads thread state state' x,
+          threads thread = Some state ->
+          S.step S.globalenv state (S.TEMemory (S.MemoryEvents.TEFree x)) state' ->
+          MM.memory_step M G (MM.MFree thread x) G' ->
+          system_step
+            {| sys_graph := G; sys_threads := threads |}
+            WSTau
+            {| sys_graph := G';
+               sys_threads := update_thread thread (Some state') threads |}
+
+    | Step_Start :
+        forall G threads thread new_thread state state' new_state info,
+          threads thread = Some state ->
+          threads new_thread = None ->
+          S.step S.globalenv state (S.TEStart new_thread info) state' ->
+          S.start_state info new_state ->
+          system_step
+            {|
+              sys_graph := G;
+              sys_threads := threads
+            |}
+            WSTau
+            {|
+              sys_graph := G;
+              sys_threads := add_thread new_thread new_state (update_thread thread (Some state') threads)
+            |}
+            .
+
+
+    (*************************************************************)
+    (* Initial system state                                      *)
+    (*************************************************************)
+
+    Parameter initial_execution : execution -> Prop.
+
+    Parameter main_thread : Ev.thread_id.
+
+    Inductive initial_system_state : system_state -> Prop :=
+    | Initial_System_State :
+        forall
+          G
+          state,
+
+          initial_execution G ->
+
+          S.initial_state state ->
+
+          initial_system_state
+
+            {|
+              sys_graph := G;
+
+              sys_threads :=
+                fun thread =>
+                  if thread_id_eq_dec thread main_thread
+                  then Some state
+                  else None
+            |}.
+
+    Definition final_system_state
+        (system : system_state)
+        (result : S.result)
+        : Prop :=
+
+      exists state,
+
+        sys_threads system main_thread =
+          Some state /\
+
+        S.final_state
+          state
+          result.
+
+    Definition tau_step
+        (system system' : system_state)
+        : Prop :=
+
+      system_step
+        system
+        WSTau
+        system'.
+
+    End WithMemoryModel.
+
+  End WholeSystem.
+
+End Composition.
