rocq_proofs/thread_semantics.v
@@ -1,0 +1,83 @@
+From hahn Require Import Hahn.
+
+Require Import Events.
+Require Import value.
+Require Import memory_model.
+
+Set Implicit Arguments.
+
+Module ThreadMemoryEvents
+    (Ev : Events ConcreteValue).
+
+  Inductive thread_mem_event : Type :=
+  | TERead :
+      Ev.location ->
+      Ev.mode ->
+      ConcreteValue.t ->
+      thread_mem_event
+  | TEWrite :
+      Ev.location ->
+      Ev.mode ->
+      ConcreteValue.t ->
+      thread_mem_event
+  | TEMalloc :
+      Ev.location ->
+      thread_mem_event
+  | TEFree :
+      Ev.location ->
+      thread_mem_event.
+
+End ThreadMemoryEvents.
+
+Module Type ThreadSemantics
+    (Ev : Events ConcreteValue).
+
+  Module Import MemoryEvents := ThreadMemoryEvents Ev.
+
+  Parameter state : Type.
+  Parameter genv : Type.
+  Parameter external_event : Type.
+  Parameter start_info : Type.
+  Parameter result : Type.
+
+  Inductive thread_event : Type :=
+  | TEExternal :
+      external_event ->
+      thread_event
+  | TEMemory :
+      thread_mem_event ->
+      thread_event
+  | TETau :
+      thread_event
+  | TEStart :
+      Ev.thread_id ->
+      start_info ->
+      thread_event
+  | TEExit :
+      thread_event.
+
+  Parameter globalenv :
+    genv.
+
+  Parameter step :
+    genv ->
+    state ->
+    thread_event ->
+    state ->
+    Prop.
+
+  Parameter initial_state :
+    state ->
+    Prop.
+
+  Parameter start_state :
+    start_info ->
+    state ->
+    Prop.
+
+  Parameter final_state :
+    state ->
+    result ->
+    Prop.
+
+End ThreadSemantics.
